language_formal/spark2014_semantics/wellformedness.v
@@ -17,23 +17,31 @@ Require Export semantics.
 (** this is used by the type system to check whether types are consistent on both sides
      of binary operators, and return either the result type or None if their types are not consistent
 *)
-Definition binop_type (op: binary_operation) (x y: typ): option typ := 
+Definition binop_type (op: binary_operation) (t1 t2: typ): option typ := 
     match op with 
     | Ceq | Cne  => 
-        match x, y with
+        match t1, t2 with
         | Tint, Tint => Some Tbool
         | _, _ => None
         end
     | Oand | Oor =>
-        match x, y with
+        match t1, t2 with
         | Tbool, Tbool => Some Tbool
         | _, _ => None
         end
     | Oadd | Osub | Omul | Odiv =>
-        match x, y with
+        match t1, t2 with
         | Tint, Tint => Some Tint
         | _, _ => None
         end
+    end.
+
+Definition unop_type (op: unary_operation) (t: typ): option typ := 
+    match op with 
+    | Onot => match t with
+              | Tbool => Some Tbool
+              | _ => None
+              end
     end.
 
 (** * Well-Typed *)
@@ -59,7 +67,7 @@ Inductive well_typed_expr: symtb -> expr -> typ -> Prop :=
         well_typed_expr tb (Eunop ast_num op e) Tbool.
 
 
-(** ** Well-typed commands *)
+(** ** Well-typed statements *)
 (**
     - general type checking;
 *)
@@ -80,6 +88,385 @@ Inductive well_typed_stmt: symtb -> stmt  -> Prop :=
         well_typed_expr tb b Tbool ->
         well_typed_stmt tb c ->
         well_typed_stmt tb (Swhile ast_num b c).
+
+
+(* in our formalization framework, all names used in the SPARK programs are 
+    formalized as integer numbers, for example, variables, function/procedure names
+    and types are all represented as distinguishable integer numbers;
+    here I hard code that number "1" representing type "Tint", and "2" representing "Tbool";
+*)
+Inductive type_map: typenum -> typ -> Prop :=
+    | T1 : type_map 1 Tint
+    | T2: type_map 2 Tbool.
+
+Inductive well_typed_decl: symtb -> local_declaration -> symtb -> Prop :=
+    | WT_Decl0: forall d x t tb,
+        x = d.(local_ident) ->
+        type_map d.(local_typenum) t ->
+        None = d.(local_init) ->
+        well_typed_decl tb d ((x, (InOut, t)) :: tb) (* the declared variables have in/out mode *)
+    | WT_Decl1: forall d x t i tb,
+        x = d.(local_ident) ->
+        type_map d.(local_typenum) t ->
+        Some i = d.(local_init) -> 
+        well_typed_expr tb i t -> (* the type of the initialization value should be consistent with the declared variable's type *)
+        well_typed_decl tb d ((x, (InOut, t)) :: tb).
+
+
+Inductive well_typed_decls: symtb -> list local_declaration -> symtb -> Prop :=
+    | WT_Decls_Empty: forall tb,
+        well_typed_decls tb nil tb
+    | WT_Decls: forall tb d tb'0 tl tb',
+        well_typed_decl tb d tb'0 ->
+        well_typed_decls tb'0 tl tb' ->
+        well_typed_decls tb (d :: tl) tb'.
+
+Inductive well_typed_proc_body: symtb -> procedure_body -> Prop :=
+    | WT_Proc_Body: forall tb f tb',
+        well_typed_decls tb f.(proc_loc_idents) tb' ->
+        well_typed_stmt tb' f.(proc_body) ->
+        well_typed_proc_body tb f.
+
+Inductive well_typed_subprogram: symtb -> subprogram -> Prop :=
+    | WT_Proc: forall tb f ast_num,
+        well_typed_proc_body tb f ->
+        well_typed_subprogram tb (Sproc ast_num f).
+
+(* =============================== *)
+
+(** functional semantics for type system *)
+
+Function f_well_typed_expr (tb: symtb) (e: expr): option typ := 
+    match e with
+    | Econst _ (Ointconst n) => Some Tint
+    | Econst _ (Oboolconst n) => Some Tbool
+    | Evar _ x =>
+        match (lookup x tb) with
+        | Some (m, t) => Some t
+        | None => None
+        end
+    | Ebinop _ op e1 e2 =>
+        match (f_well_typed_expr tb e1) with
+        | Some t1 => 
+            match (f_well_typed_expr tb e2) with
+            | Some t2 => binop_type op t1 t2
+            | None => None
+            end
+        | None => None
+        end   
+    | Eunop _ op e => 
+        match f_well_typed_expr tb e with
+        | Some t => unop_type op t
+        | None => None
+        end
+    end.
+
+Function f_typ_equal (t1: typ) (t2: typ): bool :=
+    match t1, t2 with
+    | Tint, Tint => true
+    | Tbool, Tbool => true
+    | _, _ => false
+    end.
+
+Function f_well_typed_stmt (tb: symtb) (c: stmt): bool :=
+    match c with
+    | Sassign ast_num x e =>
+        match (f_well_typed_expr tb e) with
+        | Some t1 => 
+            match lookup x tb with
+            | Some (m, t2) => (f_typ_equal t1 t2)
+            | None => false
+            end
+        | None => false
+        end
+    | Sseq ast_num c1 c2 =>
+        match f_well_typed_stmt tb c1 with
+        | true => f_well_typed_stmt tb c2
+        | false => false
+        end
+    | Sifthen ast_num b c =>
+        match f_well_typed_expr tb b with
+        | Some Tbool => f_well_typed_stmt tb c
+        | _ => false
+        end
+    | Swhile ast_num b c =>
+        match f_well_typed_expr tb b with
+        | Some Tbool => f_well_typed_stmt tb c
+        | _ => false
+        end
+    end.
+
+
+(** in the SPARK formalization, I use number to represent identifier, type and so on, 
+    here "1" represent type Tint, and "2" represent type Tbool;
+*)
+Function f_type_map (n: typenum): option typ :=
+    match n with
+    | 1 => Some Tint
+    | 2 => Some Tbool
+    | _ => None
+    end.
+
+Function f_well_typed_decl (tb: symtb) (d: local_declaration): option symtb :=
+    match f_type_map d.(local_typenum) with
+    | Some t =>
+        match d.(local_init) with
+        | Some i => 
+            match f_well_typed_expr tb i with
+            | Some t' => if f_typ_equal t t' then Some ((d.(local_ident), (InOut, t)) :: tb) else None
+            | None => None
+            end
+        | None => Some ((d.(local_ident), (InOut, t)) :: tb)
+        end
+    | None => None
+    end.
+
+(*
+Inductive well_typed_subprogram: symtb -> subprogram -> Prop :=
+    | WT_Proc: forall tb f ast_num,
+        well_typed_proc_body tb f ->
+        well_typed_subprogram tb (Sproc ast_num f).
+*)
+Function f_well_typed_decls (tb: symtb) (ds: list local_declaration): option symtb :=
+    match ds with
+    | d :: tl => 
+        match f_well_typed_decl tb d with
+        | Some tb' => f_well_typed_decls tb' tl
+        | None => None
+        end
+    | nil => Some tb
+    end.
+
+Function f_well_typed_proc_body (tb: symtb) (f: procedure_body): bool :=
+    match f_well_typed_decls tb f.(proc_loc_idents) with
+    | Some tb' => f_well_typed_stmt tb' f.(proc_body)
+    | None => false
+    end.
+
+Function f_well_typed_subprogram (tb: symtb) (p: subprogram): bool :=
+    match p with
+    | Sproc ast_num f => f_well_typed_proc_body tb f
+    end.
+
+(* =============================== *)
+
+(** Semantical equivalence between relational and functional semantics for type system *)
+
+Lemma f_well_typed_expr_correct: forall tb e t,
+    f_well_typed_expr tb e = Some t ->
+    well_typed_expr tb e t.
+Proof.
+    intros tb e.
+    functional induction (f_well_typed_expr tb e);
+    intros t'0 h1;
+    inversion h1; subst;
+    try constructor.
+  - econstructor.
+    apply e1.
+  - specialize (IHo _ e3).
+    specialize (IHo0 _ e4).
+    econstructor.
+    apply IHo.
+    destruct t1, t2, op; 
+    inversion h1; auto.
+    destruct t1, t2, op;
+    inversion h1; auto.
+  - specialize (IHo _ e2).
+    destruct t, t'0, op; inversion h1.
+    constructor.
+    assumption.
+Qed.
+
+Lemma f_well_typed_expr_complete: forall tb e t,
+    well_typed_expr tb e t ->
+    f_well_typed_expr tb e = Some t.
+Proof.
+    intros tb e t h1.
+    induction h1;
+    try constructor;
+    simpl.
+  - rewrite H. reflexivity.
+  - rewrite IHh1_1, IHh1_2.
+    assumption.
+  - rewrite IHh1.
+    destruct op; auto.
+Qed.
+
+Lemma f_well_typed_stmt_correct: forall tb c,
+    f_well_typed_stmt tb c = true ->
+    well_typed_stmt tb c.
+Proof.
+    intros tb c.
+    functional induction (f_well_typed_stmt tb c);
+    intros h1;
+    try match goal with
+    | [h: false = true |- _] => inversion h
+    end.
+  - econstructor.
+    apply e2.
+    specialize (f_well_typed_expr_correct _ _ _ e1); intros h2.
+    destruct t1, t2; inversion h1;
+    auto.
+  - specialize (IHb e0).
+    specialize (IHb0 h1).
+    constructor; assumption.
+  - specialize (IHb h1).
+    constructor; auto.
+    specialize (f_well_typed_expr_correct _ _ _ e0); intros h2.
+    assumption.
+  - specialize (IHb h1).
+    constructor; auto.
+    specialize (f_well_typed_expr_correct _ _ _ e0); intros h2.
+    assumption.
+Qed.
+
+Lemma f_well_typed_stmt_complete: forall tb c,
+    well_typed_stmt tb c ->
+    f_well_typed_stmt tb c = true.
+Proof.
+    intros tb c h1.
+    induction h1; simpl.
+  - specialize (f_well_typed_expr_complete _ _ _ H0); intros h2.
+    rewrite h2.
+    rewrite H.
+    destruct t; auto.
+  - rewrite IHh1_1, IHh1_2.
+    reflexivity.
+  - specialize (f_well_typed_expr_complete _ _ _ H); intros h2.
+    rewrite h2, IHh1.
+    reflexivity.
+  - specialize (f_well_typed_expr_complete _ _ _ H); intros h2.
+    rewrite h2, IHh1.
+    reflexivity.
+Qed.
+
+Lemma type_map_equal: forall n t,
+    f_type_map n = Some t <-> type_map n t.
+Proof.
+    intros n t; split;
+    intros h1.
+  - functional induction (f_type_map n);
+    inversion h1; subst;
+    constructor.
+  - induction h1;
+    simpl; auto.
+Qed.
+
+
+Lemma f_well_typed_decl_correct: forall tb d tb',
+    f_well_typed_decl tb d = Some tb' ->
+    well_typed_decl tb d tb'.
+Proof.
+    intros tb d.
+    functional induction f_well_typed_decl tb d;
+    intros tb' h1;
+    inversion h1; subst.
+  - eapply WT_Decl1; auto.
+    + apply type_map_equal; 
+      assumption.
+    + symmetry in e0; apply e0.
+    + specialize (f_well_typed_expr_correct _ _ _ e1); intros h2.
+      destruct t, t'; inversion e2; auto.
+  - eapply WT_Decl0; auto.
+    apply type_map_equal; assumption.
+Qed.
+
+Lemma f_well_typed_decl_complete: forall tb d tb',
+    well_typed_decl tb d tb' ->
+    f_well_typed_decl tb d = Some tb'.
+Proof.
+    intros tb d tb' h1.
+    induction h1;
+    specialize (type_map_equal (local_typenum d) t); intros h2;
+    destruct h2 as [h3 h4];
+    specialize (h4 H0);
+    unfold f_well_typed_decl;
+    rewrite h4; rewrite <- H1; rewrite <- H.
+  - reflexivity.
+  - specialize (f_well_typed_expr_complete _ _ _ H2); intros h2.
+    rewrite h2.
+    destruct t; simpl; auto.
+Qed.
+
+
+Lemma f_well_typed_decls_correct: forall tb ds tb',
+    f_well_typed_decls tb ds = Some tb' ->
+    well_typed_decls tb ds tb'.
+Proof.
+    intros tb ds.
+    functional induction (f_well_typed_decls tb ds);
+    intros tb'0 h1.
+  - specialize (IHo _ h1).
+    econstructor.
+    specialize (f_well_typed_decl_correct _ _ _ e0); intros h2.
+    apply h2.
+    assumption.
+  - inversion h1.
+  - inversion h1; subst.
+    constructor.
+Qed.
+
+Lemma f_well_typed_decls_complete: forall tb ds tb',
+    well_typed_decls tb ds tb' ->
+    f_well_typed_decls tb ds = Some tb'.
+Proof.
+    intros tb ds tb' h1.
+    induction h1.
+  - simpl; auto.
+  - specialize (f_well_typed_decl_complete _ _ _ H); intros h2.
+    simpl.
+    rewrite h2. assumption.
+Qed.
+
+
+Lemma f_well_typed_proc_body_correct: forall tb f,
+    f_well_typed_proc_body tb f = true ->
+    well_typed_proc_body tb f.
+Proof.
+    intros tb f h1.
+    functional induction (f_well_typed_proc_body tb f).
+  - econstructor.
+    specialize (f_well_typed_decls_correct _ _ _ e); intros h2.
+    apply h2.
+    specialize (f_well_typed_stmt_correct _ _ h1); intros h2.
+    assumption.
+  - inversion h1.
+Qed.
+
+Lemma f_well_typed_proc_body_complete: forall tb f,
+    well_typed_proc_body tb f ->
+    f_well_typed_proc_body tb f = true.
+Proof.
+    intros tb f h1.
+    induction h1.
+    specialize (f_well_typed_decls_complete _ _ _ H); intros h1.
+    specialize (f_well_typed_stmt_complete _ _ H0); intros h2.
+    unfold f_well_typed_proc_body.
+    rewrite h1, h2.
+    auto.
+Qed.
+
+Lemma f_well_typed_subprogram_correct: forall tb p,
+    f_well_typed_subprogram tb p = true ->
+    well_typed_subprogram tb p.
+Proof.
+    intros tb p h1.
+    functional induction (f_well_typed_subprogram tb p).
+    specialize (f_well_typed_proc_body_correct _ _ h1); intros h2.
+    constructor.
+    assumption.
+Qed.
+
+Lemma f_well_typed_subprogram_complete: forall tb p,
+    well_typed_subprogram tb p ->
+    f_well_typed_subprogram tb p = true.
+Proof.
+    intros tb p h1.
+    induction h1.
+    specialize (f_well_typed_proc_body_complete _ _ H); intros h1.
+    simpl. assumption.
+Qed.
+
 
 (* =============================== *)
 
@@ -169,6 +556,40 @@ Inductive well_defined_stmt: mode_map -> stmt -> mode_map -> Prop :=
         well_defined_expr m b ->
         well_defined_stmt m c m' ->
         well_defined_stmt m (Swhile ast_num b c) m.
+
+
+(** in our current SPARK subset, we only consider Int and Bool types, which have no default initialization values,
+     so for any declared variable, if it's declared without initialization expression, then it's uninitialized;
+*)
+Inductive well_defined_decl: mode_map -> local_declaration -> mode_map -> Prop :=
+    | WD_Decl0: forall d x m,
+        x = d.(local_ident) ->
+        None = d.(local_init) ->
+        well_defined_decl m d ((x, (Uninit, InOut)) :: m) 
+    | WD_Decl1: forall d x i m,
+        x = d.(local_ident) ->
+        Some i = d.(local_init) ->
+        well_defined_expr m i ->
+        well_defined_decl m d ((x, (Init, InOut)) :: m).
+
+Inductive well_defined_decls: mode_map -> list local_declaration -> mode_map -> Prop :=
+    | WD_Decls_Empty: forall m,
+        well_defined_decls m nil m
+    | WD_Decls: forall m d m'0 tl m',
+        well_defined_decl m d m'0 ->
+        well_defined_decls m'0 tl m' ->
+        well_defined_decls m (d :: tl) m'.
+
+Inductive well_defined_proc_body: mode_map -> procedure_body -> mode_map -> Prop :=
+    | WD_Proc_Body: forall m f m'0 m',
+        well_defined_decls m f.(proc_loc_idents) m'0 ->
+        well_defined_stmt m'0 f.(proc_body) m' -> 
+        well_defined_proc_body m f m'.
+
+Inductive well_defined_subprogram: mode_map -> subprogram -> mode_map -> Prop :=
+    | WD_Subprogram: forall m f m' ast_num,
+        well_defined_proc_body m f m' ->        
+        well_defined_subprogram m (Sproc ast_num f) m'.
 
 (** ** Lemmas for fetching and updating initialization state *)
 Lemma update2_fetch2: forall s x m s',
@@ -422,6 +843,322 @@ Proof.
     apply IHh1; assumption.
 Qed.
 
+(* =============================== *)
+Function f_mode_mapping (tb: symtb) (s: stack): option mode_map :=
+    match tb, s with
+    | nil, nil => Some nil
+    | ((x, (md, Tbool)) :: tb'), ((x', (Value (Bool b))) :: s') => 
+        if beq_nat x x' then
+          match f_mode_mapping tb' s' with
+          | Some m => Some ((x, (Init, md)) :: m)
+          | None => None
+          end
+        else 
+          None
+    | ((x, (md, Tint)) :: tb'), ((x', (Value (Int v))) :: s') => 
+        if beq_nat x x' then
+          match f_mode_mapping tb' s' with
+          | Some m => Some ((x, (Init, md)) :: m)
+          | None => None
+          end
+        else 
+          None
+    | ((x, (md, Tbool)) :: tb'), ((x', Vundef) :: s') => 
+        if beq_nat x x' then
+          match f_mode_mapping tb' s' with
+          | Some m => Some ((x, (Uninit, md)) :: m)
+          | None => None
+          end
+        else
+          None
+    | ((x, (md, Tint)) :: tb'), ((x', Vundef) :: s') => 
+        if beq_nat x x' then
+          match f_mode_mapping tb' s' with
+          | Some m => Some ((x, (Uninit, md)) :: m)
+          | None => None
+          end
+        else
+          None
+    | _, _ => None
+    end.
+
+
+(* =============================== *)
+
+(** Functional semantics for checking whether used variables being initialized *)
+Function f_well_defined_expr (m: mode_map) (e: expr): bool :=
+    match e with
+    | Econst ast_num v => true
+    | Evar ast_num x =>
+        match fetch2 x m with
+        | Some (Init, md) => true
+        | _ => false
+        end
+    | Ebinop ast_num op e1 e2 =>
+        if (f_well_defined_expr m e1) then (f_well_defined_expr m e2) else false
+    | Eunop ast_num op e => f_well_defined_expr m e
+    end.
+
+Function f_well_defined_stmt (m: mode_map) (c: stmt): option mode_map :=
+    match c with
+    | Sassign ast_num x e =>
+        match fetch2 x m with
+        | Some (_, Out) => 
+            if f_well_defined_expr m e then update2 m x (Init, Out) else None
+        | Some (_, InOut) => 
+            if f_well_defined_expr m e then update2 m x (Init, InOut) else None
+        | _ => None
+        end
+    | Sseq ast_num c1 c2 =>
+        match f_well_defined_stmt m c1 with
+        | Some m' => f_well_defined_stmt m' c2
+        | None => None
+        end
+    | Sifthen ast_num b c =>
+        if f_well_defined_expr m b 
+        then 
+            match f_well_defined_stmt m c with
+            | Some m' => Some m
+            | None => None
+            end
+        else None
+    | Swhile ast_num b c =>
+        if f_well_defined_expr m b 
+        then 
+            match f_well_defined_stmt m c with
+            | Some m' => Some m
+            | None => None
+            end
+        else None
+    end.
+
+Function f_well_defined_decl (m: mode_map) (d: local_declaration): option mode_map :=
+    match d.(local_init) with
+    | Some i => 
+        if f_well_defined_expr m i then Some ((d.(local_ident), (Init, InOut)) :: m) else None
+    | None => Some ((d.(local_ident), (Uninit, InOut)) :: m)
+    end.
+
+Function f_well_defined_decls (m: mode_map) (ds: list local_declaration): option mode_map :=
+    match ds with
+    | d :: tl =>
+        match f_well_defined_decl m d with
+        | Some m' => f_well_defined_decls m' tl
+        | None => None
+        end
+    | nil => Some m
+    end.
+
+Function f_well_defined_proc_body (m: mode_map) (f: procedure_body): option mode_map :=
+    match f_well_defined_decls m f.(proc_loc_idents) with
+    | Some m' => f_well_defined_stmt m' f.(proc_body)
+    | None => None
+    end.
+
+Function f_well_defined_subprogram (m: mode_map) (p: subprogram): option mode_map :=
+    match p with
+    | Sproc ast_num f => f_well_defined_proc_body m f
+    end.
+
+
+(* =============================== *)
+
+(** Semantical equivalence between relational and functional semantics for initialization state checking system *)
+
+Lemma f_well_defined_expr_correct: forall m e,
+    f_well_defined_expr m e = true ->
+    well_defined_expr m e.
+Proof.
+    intros m e h1.
+    functional induction (f_well_defined_expr m e).
+  - destruct v; constructor.
+  - econstructor.
+    apply e1.
+  - inversion h1.
+  - specialize (IHb e3).
+    specialize (IHb0 h1).
+    constructor; assumption.
+  - inversion h1.
+  - specialize (IHb h1).
+    constructor; assumption.
+Qed.
+
+Lemma f_well_defined_expr_complete: forall m e,
+    well_defined_expr m e ->
+    f_well_defined_expr m e = true.
+Proof.
+    intros m e h1.
+    induction h1;
+    simpl; auto.
+  - rewrite H.
+    reflexivity.
+  - rewrite IHh1_1.
+    assumption.
+Qed.
+
+Lemma f_well_defined_stmt_correct: forall m c m',
+    f_well_defined_stmt m c = Some m' ->
+    well_defined_stmt m c m'.
+Proof.
+    intros m c.
+    functional induction (f_well_defined_stmt m c);
+    intros m'0 h1;
+    try match goal with
+    | [h: None = Some ?x |- _] => inversion h
+    end.
+  - econstructor.
+    specialize (f_well_defined_expr_correct _ _ e2); auto.
+    apply e1.
+    intuition. inversion H.
+    assumption.
+  - econstructor.
+    specialize (f_well_defined_expr_correct _ _ e2); auto.
+    apply e1.
+    intuition. inversion H.
+    assumption.
+  - specialize (IHo _ e0).
+    specialize (IHo0 _ h1).
+    econstructor.
+    apply IHo. apply IHo0.
+  - inversion h1; subst.
+    specialize (IHo _ e1).
+    econstructor.
+    specialize (f_well_defined_expr_correct _ _ e0); auto.
+    apply IHo.
+  - inversion h1; subst.
+    specialize (IHo _ e1).
+    econstructor.
+    specialize (f_well_defined_expr_correct _ _ e0); auto.
+    apply IHo.
+Qed.
+
+Lemma f_well_defined_stmt_complete: forall m c m',
+    well_defined_stmt m c m' ->
+    f_well_defined_stmt m c = Some m'.
+Proof.
+    intros m c m' h1.
+    induction h1; simpl.
+  - rewrite H0.
+    specialize (f_well_defined_expr_complete _ _ H); intros hz1.
+    rewrite hz1.
+    destruct md; auto.
+    destruct H1; auto.
+  - rewrite IHh1_1, IHh1_2.
+    reflexivity.
+  - specialize (f_well_defined_expr_complete _ _ H); intros hz1.
+    rewrite hz1, IHh1.
+    reflexivity.
+  - specialize (f_well_defined_expr_complete _ _ H); intros hz1.
+    rewrite hz1, IHh1.
+    reflexivity.
+Qed.
+
+Lemma f_well_defined_decl_correct: forall m d m',
+    f_well_defined_decl m d = Some m' ->
+    well_defined_decl m d m'.
+Proof.
+    intros m d.
+    functional induction (f_well_defined_decl m d);
+    intros m' h1;
+    inversion h1; subst.
+  - econstructor; auto.
+    symmetry in e. apply e.
+    specialize (f_well_defined_expr_correct _ _ e0); auto.
+  - econstructor; auto.
+Qed.
+
+Lemma f_well_defined_decl_complete: forall m d m',
+    well_defined_decl m d m' ->
+    f_well_defined_decl m d = Some m'.
+Proof.
+    intros m d m' h1.
+    induction h1;
+    unfold f_well_defined_decl;
+    rewrite <- H0, H.
+  - reflexivity.
+  - specialize (f_well_defined_expr_complete _ _ H1); intros hz1.
+    rewrite hz1.
+    reflexivity.
+Qed.
+
+Lemma f_well_defined_decls_correct: forall m ds m',
+    f_well_defined_decls m ds = Some m' ->
+    well_defined_decls m ds m'.
+Proof.
+    intros m ds.
+    functional induction (f_well_defined_decls m ds);
+    intros m'0 h1.
+  - specialize (IHo _ h1).
+    econstructor.
+    specialize (f_well_defined_decl_correct _ _ _ e0); intros hz1.
+    apply hz1.
+    assumption.
+  - inversion h1.
+  - inversion h1; subst.
+    constructor.
+Qed.
+
+Lemma f_well_defined_decls_complete: forall m ds m',
+    well_defined_decls m ds m' ->
+    f_well_defined_decls m ds = Some m'.
+Proof.
+    intros m ds m' h1.
+    induction h1; simpl.
+  - reflexivity.
+  - specialize (f_well_defined_decl_complete _ _ _ H); intros hz1.
+    rewrite hz1.
+    rewrite IHh1.
+    reflexivity.
+Qed.
+
+Lemma f_well_defined_proc_body_correct: forall m f m',
+    f_well_defined_proc_body m f = Some m' ->
+    well_defined_proc_body m f m'.
+Proof.
+    intros m f.
+    functional induction (f_well_defined_proc_body m f);
+    intros m'0 h1.
+  - econstructor.
+    specialize (f_well_defined_decls_correct _ _ _ e); intro hz1.
+    apply hz1.
+    specialize (f_well_defined_stmt_correct _ _ _ h1); intros hz2.
+    exact hz2.
+  - inversion h1.
+Qed.
+
+Lemma f_well_defined_proc_body_complete: forall m f m',
+    well_defined_proc_body m f m' ->
+    f_well_defined_proc_body m f = Some m'.
+Proof.
+    intros m f m' h1.
+    induction h1.
+    unfold f_well_defined_proc_body.
+    specialize (f_well_defined_decls_complete _ _ _ H); intros hz1.
+    specialize (f_well_defined_stmt_complete _ _ _ H0); intros hz2.
+    rewrite hz1, hz2.
+    reflexivity.
+Qed.
+
+Lemma f_well_defined_subprogram_correct: forall m p m',
+    f_well_defined_subprogram m p = Some m' ->
+    well_defined_subprogram m p m'.
+Proof.
+    intros m p.
+    functional induction (f_well_defined_subprogram m p);
+    intros m' h1.
+    constructor.
+    specialize (f_well_defined_proc_body_correct _ _ _ h1); auto.
+Qed.
+
+Lemma f_well_defined_subprogram_complete: forall m p m',
+    well_defined_subprogram m p m' ->
+    f_well_defined_subprogram m p = Some m'.
+Proof.
+    intros m p m' h1.
+    induction h1.
+    simpl.
+    specialize (f_well_defined_proc_body_complete _ _ _ H); auto.
+Qed.
 
 
 (* = = = = = = = = = = = = = = = = = = = = = = = = = = = = = = = = *)
@@ -444,6 +1181,7 @@ Definition get_ast_num_stmt (c: stmt): astnum :=
     | (Sifthen ast_num b c) => ast_num
     | (Swhile ast_num b c) => ast_num
     end.
+
 
 Definition max_num := astnum.
 
@@ -512,6 +1250,510 @@ Inductive ast_num_inc_stmt: stmt -> max_num -> Prop :=
         ast_num_inc_stmt (Swhile ast_num b c) max2.
 
 
+Inductive ast_num_inc_decl: local_declaration -> max_num -> Prop :=
+    | Inc_Decl0: forall n0 d i max n1,
+        n0 = d.(local_astnum) ->
+        Some i = d.(local_init) ->
+        ast_num_inc_expr i max ->
+        get_ast_num_expr i = n1 ->
+        n0 < n1 ->
+        ast_num_inc_decl d max
+    | Inc_Decl1: forall n d,
+        n = d.(local_astnum) ->
+        None = d.(local_init) ->
+        ast_num_inc_decl d n.
+
+Inductive ast_num_inc_decls: list local_declaration -> max_num -> Prop :=
+    | Inc_Decls_Empty: forall n, 
+        ast_num_inc_decls nil n
+    | Inc_Decls1: forall d n,
+        ast_num_inc_decl d n ->
+        ast_num_inc_decls (d :: nil) n
+    | Inc_Decls2: forall d1 n1 d2 n2 tl,
+        ast_num_inc_decl d1 n1 ->
+        n1 < d2.(local_astnum) ->
+        ast_num_inc_decls (d2 :: tl) n2 ->
+        ast_num_inc_decls (d1 :: (d2 :: tl)) n2.
+
+Inductive ast_num_inc_proc_body: procedure_body -> max_num -> Prop :=
+    | Inc_Proc_Body0: forall f max,
+        nil = f.(proc_loc_idents) ->
+        ast_num_inc_stmt f.(proc_body) max ->
+        f.(proc_astnum) < get_ast_num_stmt f.(proc_body) ->
+        ast_num_inc_proc_body f max
+    | Inc_Proc_Body1: forall d tl f max1 max2,
+        (d :: tl) = f.(proc_loc_idents) ->
+        ast_num_inc_decls f.(proc_loc_idents) max1 ->
+        ast_num_inc_stmt f.(proc_body) max2 ->
+        f.(proc_astnum) < d.(local_astnum) ->
+        f.(proc_astnum) < get_ast_num_stmt f.(proc_body) ->
+        max1 < get_ast_num_stmt f.(proc_body) ->
+        ast_num_inc_proc_body f max2.
+
+Inductive ast_num_inc_subprogram: subprogram -> max_num -> Prop :=
+    | Inc_Subprogram: forall f n ast_num,
+        ast_num < f.(proc_astnum) ->
+        ast_num_inc_proc_body f n ->
+        ast_num_inc_subprogram (Sproc ast_num f) n.
+
+(*************************************************)
+
+(** Function to test whether ast numbers labled for each ast node are increasing in
+    depth-first way;
+*)
+
+(** To import the function "leb" from the library Arith.Compare_dec; *)
+Require Import Arith.Compare_dec.
+
+Function f_ast_num_inc_expr (e: expr): option max_num :=
+    match e with
+    | Econst ast_num n => Some ast_num
+    | Evar ast_num x => Some ast_num
+    | Ebinop ast_num op e1 e2 =>
+        if (leb (get_ast_num_expr e1) ast_num) || (leb (get_ast_num_expr e2) ast_num) then
+          None
+        else
+          match f_ast_num_inc_expr e1 with
+          | Some n1 => 
+              match f_ast_num_inc_expr e2 with
+              | Some n2 => if leb (get_ast_num_expr e2) n1 then None else Some n2
+              | None => None
+              end
+          | None => None
+          end
+    | Eunop ast_num op e =>
+        if leb (get_ast_num_expr e) ast_num then
+          None
+        else
+          f_ast_num_inc_expr e
+    end.
+  
+Function f_ast_num_inc_stmt (c: stmt): option max_num :=
+    match c with
+    | Sassign ast_num x e =>
+        if leb (get_ast_num_expr e) ast_num then None else f_ast_num_inc_expr e
+    | Sseq ast_num c1 c2 =>
+        if (leb (get_ast_num_stmt c1) ast_num) || (leb (get_ast_num_stmt c2) ast_num) then
+          None
+        else
+          match f_ast_num_inc_stmt c1 with
+          | Some n1 =>
+              match f_ast_num_inc_stmt c2 with
+              | Some n2 => if leb (get_ast_num_stmt c2) n1 then None else Some n2
+              | None => None
+              end
+          | None => None
+          end
+    | Sifthen ast_num b c =>
+        if (leb (get_ast_num_expr b) ast_num) || (leb (get_ast_num_stmt c) ast_num) then
+          None
+        else
+          match f_ast_num_inc_expr b with
+          | Some n1 => 
+              match f_ast_num_inc_stmt c with
+              | Some n2 => if leb (get_ast_num_stmt c) n1 then None else Some n2
+              | None => None
+              end
+          | None => None
+          end
+    | Swhile ast_num b c =>
+        if (leb (get_ast_num_expr b) ast_num) || (leb (get_ast_num_stmt c) ast_num) then
+          None
+        else
+          match f_ast_num_inc_expr b with
+          | Some n1 => 
+              match f_ast_num_inc_stmt c with
+              | Some n2 => if leb (get_ast_num_stmt c) n1 then None else Some n2
+              | None => None
+              end
+          | None => None
+          end
+    end.
+
+Function f_ast_num_inc_decl (d: local_declaration): option max_num :=
+    match d.(local_init) with
+    | Some i => 
+        match f_ast_num_inc_expr i with
+        | Some n => if leb (get_ast_num_expr i) d.(local_astnum) then None else Some n
+        | None => None
+        end
+    | None => Some d.(local_astnum)
+    end.
+
+Function f_ast_num_inc_decls (ds: list local_declaration): option max_num :=
+    match ds with
+    | nil => Some 0 (* 0 is the default value for maximum ast number of empty declarations *)
+    | d1 :: ds1 =>
+        match f_ast_num_inc_decl d1 with
+        | Some n1 =>
+            match ds1 with
+            | nil => Some n1
+            | d2 :: ds2 => 
+                if leb d2.(local_astnum) n1 then None else f_ast_num_inc_decls ds1
+            end
+        | None => None
+        end
+    end.
+
+Function f_ast_num_inc_proc_body (f: procedure_body): option max_num :=
+    match f.(proc_loc_idents) with
+    | nil => 
+        if leb (get_ast_num_stmt f.(proc_body)) f.(proc_astnum) 
+        then None 
+        else f_ast_num_inc_stmt f.(proc_body)
+    | d :: ds' => 
+        if leb d.(local_astnum) f.(proc_astnum) || leb (get_ast_num_stmt f.(proc_body)) f.(proc_astnum) 
+        then None
+        else
+          match f_ast_num_inc_decls f.(proc_loc_idents) with
+          | Some n1 =>
+              if leb (get_ast_num_stmt f.(proc_body)) n1 
+              then None
+              else f_ast_num_inc_stmt f.(proc_body)
+          | None => None
+          end
+    end.
+
+
+Function f_ast_num_inc_subprogram (p: subprogram): option max_num :=
+    match p with
+    | Sproc ast_num f =>
+        if leb f.(proc_astnum) ast_num 
+        then None
+        else f_ast_num_inc_proc_body f
+    end.
+
+(* ===================================== *)
+
+(** Semantical equivalence between relational and functional one for checking that ast number  
+    are unique in the ast tree;
+*)
+Lemma expr_ast_num_exists: forall e,
+    exists n, get_ast_num_expr e = n.
+Proof.
+    intros.
+    destruct e; simpl;
+    match goal with
+    | [|- exists n, ?a = n] => exists a; reflexivity
+    end.
+Qed.
+
+Lemma stmt_ast_num_exists: forall c,
+    exists n, get_ast_num_stmt c = n.
+Proof.
+    intros.
+    destruct c; simpl;
+    match goal with
+    | [|- exists n, ?a = n] => exists a; reflexivity
+    end.
+Qed.
+
+Lemma leb_false_lt: forall x n y,
+    leb x n || leb y n = false ->
+    n < x /\ n < y.
+Proof.
+    intros.
+    unfold "||" in H.
+    remember (leb x n) as z.
+    destruct z. inversion H.
+    symmetry in Heqz.
+    specialize (leb_complete_conv _ _ Heqz); intros hz1.
+    specialize (leb_complete_conv _ _ H); intros hz2.
+    split; auto.
+Qed.
+
+Lemma f_ast_num_inc_expr_correct: forall e max,
+    f_ast_num_inc_expr e = Some max ->
+    ast_num_inc_expr e max.
+Proof.
+    intros e.
+    functional induction (f_ast_num_inc_expr e);
+    intros max h1;
+    try match goal with
+    | [h: None = Some ?n |- _] => inversion h
+    end.
+  - inversion h1; subst.
+    constructor.
+  - inversion h1; subst.
+    constructor.
+  - inversion h1; subst.
+    specialize (IHo _ e4).
+    specialize (IHo0 _ e5).
+    specialize (expr_ast_num_exists e1); intros hz1.
+    destruct hz1.
+    specialize (expr_ast_num_exists e2); intros hz2.
+    destruct hz2.
+    rewrite H, H0 in *.
+    specialize (leb_complete_conv _ _ e6); intros hz3.
+    specialize (leb_false_lt _ _ _ e3); intros hz4.
+    destruct hz4 as [hz4 hz5].
+    econstructor.
+    exact IHo.
+    exact IHo0.
+    apply H. apply H0.
+    assumption. assumption.
+    assumption.
+  - specialize (IHo _ h1).
+    specialize (leb_complete_conv _ _ e2); intros hz1.
+    econstructor; intuition.
+Qed.
+
+Lemma f_ast_num_inc_expr_complete: forall e max,
+    ast_num_inc_expr e max ->
+    f_ast_num_inc_expr e = Some max.
+Proof.
+    intros e max h1.
+    induction h1; 
+    simpl; auto.
+  - rewrite H, H0 in *.
+    specialize (leb_correct_conv _ _ H1); intros hz1.
+    specialize (leb_correct_conv _ _ H2); intros hz2.
+    specialize (leb_correct_conv _ _ H3); intros hz3.
+    rewrite hz1, hz2, IHh1_1, IHh1_2.
+    simpl.
+    rewrite hz3.
+    reflexivity.
+  - rewrite H, IHh1 in *.
+    specialize (leb_correct_conv _ _ H0); intros hz1.
+    rewrite hz1.
+    reflexivity.
+Qed.
+
+Lemma f_ast_num_inc_stmt_correct: forall c max,
+    f_ast_num_inc_stmt c = Some max ->
+    ast_num_inc_stmt c max.
+Proof.
+    intros c.
+    functional induction (f_ast_num_inc_stmt c);
+    intros max h1;
+    try match goal with
+    | [h: None = Some ?n |- _] => inversion h
+    end.
+  - econstructor; intuition.
+    specialize (f_ast_num_inc_expr_correct _ _ h1); auto.
+    specialize (leb_complete_conv _ _ e1); auto.
+  - inversion h1; subst.
+    specialize (IHo _ e1).
+    specialize (IHo0 _ e2).
+    specialize (leb_complete_conv _ _ e3); intros hz1.
+    specialize (leb_false_lt _ _ _ e0); intros hz2.
+    destruct hz2 as [hz2 hz3].
+    econstructor; auto.
+    exact IHo.
+    intuition. intuition. intuition.
+  - inversion h1; subst.
+    specialize (IHo _ e2).
+    specialize (leb_complete_conv _ _ e3); intros hz1.
+    specialize (leb_false_lt _ _ _ e0); intros hz2.
+    destruct hz2 as [hz2 hz3].
+    econstructor; auto.
+    specialize (f_ast_num_inc_expr_correct _ _ e1); intros hz4.
+    exact hz4.
+    intuition. intuition. intuition.
+  - inversion h1; subst.
+    specialize (IHo _ e2).
+    specialize (leb_complete_conv _ _ e3); intros hz1.
+    specialize (leb_false_lt _ _ _ e0); intros hz2.
+    destruct hz2 as [hz2 hz3].
+    econstructor; auto.
+    specialize (f_ast_num_inc_expr_correct _ _ e1); intros hz4.
+    exact hz4.
+    intuition. intuition. intuition.
+Qed.
+
+Lemma f_ast_num_inc_stmt_complete: forall c max,
+    ast_num_inc_stmt c max ->
+    f_ast_num_inc_stmt c = Some max.
+Proof.
+    intros c max h1.
+    induction h1;
+    simpl.
+  - specialize (leb_correct_conv _ _ H1); intros hz1.
+    rewrite H0, hz1.
+    specialize (f_ast_num_inc_expr_complete _ _ H); auto.
+  - rewrite H, H0 in *.
+    specialize (leb_correct_conv _ _ H1); intros hz1.
+    specialize (leb_correct_conv _ _ H2); intros hz2.
+    specialize (leb_correct_conv _ _ H3); intros hz3.
+    rewrite hz1, hz2, IHh1_1, IHh1_2, hz3.
+    simpl. reflexivity.
+  - rewrite H0, H1 in *.
+    specialize (leb_correct_conv _ _ H2); intros hz1.
+    specialize (leb_correct_conv _ _ H3); intros hz2.
+    specialize (leb_correct_conv _ _ H4); intros hz3.    
+    specialize (f_ast_num_inc_expr_complete _ _ H); intros hz4.
+    rewrite hz1, hz2, hz4, IHh1, hz3.
+    simpl; auto.
+  - rewrite H0, H1 in *.
+    specialize (leb_correct_conv _ _ H2); intros hz1.
+    specialize (leb_correct_conv _ _ H3); intros hz2.
+    specialize (leb_correct_conv _ _ H4); intros hz3.    
+    specialize (f_ast_num_inc_expr_complete _ _ H); intros hz4.
+    rewrite hz1, hz2, hz4, IHh1, hz3.
+    simpl; auto.
+Qed.
+
+Lemma f_ast_num_inc_decl_correct: forall d max,
+    f_ast_num_inc_decl d = Some max ->
+    ast_num_inc_decl d max.
+Proof.
+    intros d.
+    functional induction (f_ast_num_inc_decl d);
+    intros max h1;
+    try match goal with
+    | [h: None = Some ?n |- _] => inversion h
+    end.
+  - inversion h1; subst.
+    specialize (f_ast_num_inc_expr_correct _ _ e0); intros hz1.
+    specialize (leb_complete_conv _ _ e1); intros hz2.
+    econstructor; auto.
+    symmetry in e; exact e.
+    assumption. intuition.
+  - inversion h1; subst.
+    constructor; intuition.
+Qed.
+
+Lemma f_ast_num_inc_decl_complete: forall d max,
+    ast_num_inc_decl d max ->
+    f_ast_num_inc_decl d = Some max.
+Proof.
+    intros d max h1.
+    induction h1;
+    unfold f_ast_num_inc_decl.
+  - symmetry in H, H0.
+    rewrite H0, H, H2.
+    specialize (f_ast_num_inc_expr_complete _ _ H1); intros hz1.
+    specialize (leb_correct_conv _ _ H3); intros hz2.
+    rewrite hz1, hz2.
+    reflexivity.
+  - rewrite <- H0.
+    intuition.
+Qed.
+
+(** for declaration part with at least one declaration definition; *)
+Lemma f_ast_num_inc_decls_correct: forall tl d max,
+    f_ast_num_inc_decls (d :: tl) = Some max ->
+    ast_num_inc_decls (d :: tl) max.
+Proof.
+    induction tl;
+    intros d max h1.
+  - constructor.
+    simpl in h1.
+    remember (f_ast_num_inc_decl d) as x.
+    destruct x.
+    + inversion h1; subst.
+      symmetry in Heqx. 
+      specialize (f_ast_num_inc_decl_correct _ _ Heqx); auto.
+    + inversion h1.
+  - simpl in h1.
+    remember (f_ast_num_inc_decl d) as x.
+    symmetry in Heqx.
+    destruct x.
+    + remember (leb (local_astnum a) m) as y.
+      symmetry in Heqy.
+      destruct y. inversion h1.
+      specialize (f_ast_num_inc_decl_correct _ _ Heqx); intros hz1.
+      specialize (leb_complete_conv _ _ Heqy); intros hz2.
+      econstructor.
+      exact hz1. exact hz2.
+      specialize (IHtl _ _ h1).
+      assumption.
+    + inversion h1.
+Qed.
+
+Lemma f_ast_num_inc_decls_complete: forall tl d max,
+    ast_num_inc_decls (d :: tl) max ->
+    f_ast_num_inc_decls (d :: tl) = Some max.
+Proof.
+    induction tl;
+    intros d max h1;
+    inversion h1; subst;
+    simpl.
+  - specialize (f_ast_num_inc_decl_complete _ _ H0); intros hz1.
+    rewrite hz1.
+    reflexivity.
+  - specialize (IHtl _ _ H5).
+    specialize (f_ast_num_inc_decl_complete _ _ H2); intros hz1.
+    specialize (leb_correct_conv _ _ H4); intros hz2.
+    rewrite hz1, hz2.
+    assumption.
+Qed.
+
+Lemma f_ast_num_inc_proc_body_correct: forall f max,
+    f_ast_num_inc_proc_body f = Some max ->
+    ast_num_inc_proc_body f max.
+Proof.
+    intros f.
+    functional induction (f_ast_num_inc_proc_body f);
+    intros max h1;
+    try match goal with
+    | [h: None = Some ?n |- _] => inversion h
+    end.
+  - econstructor; auto.
+    specialize (f_ast_num_inc_stmt_correct _ _ h1); auto.
+    specialize (leb_complete_conv _ _ e0); auto.
+  - rewrite e in *.
+    specialize (f_ast_num_inc_decls_correct _ _ _ e1); intros hz1.
+    specialize (f_ast_num_inc_stmt_correct _ _ h1); intros hz2.
+    specialize (leb_false_lt _ _ _ e0); intros hz3.
+    destruct hz3 as [hz3 hz4].
+    specialize (leb_complete_conv _ _ e2); intros hz5.
+    eapply Inc_Proc_Body1.
+    symmetry in e; exact e.
+    rewrite e; exact hz1.
+    assumption. assumption.
+    assumption. assumption.
+Qed.
+
+Lemma f_ast_num_inc_proc_body_complete: forall f max,
+    ast_num_inc_proc_body f max ->
+    f_ast_num_inc_proc_body f = Some max.
+Proof.
+    intros f max h1.
+    induction h1;
+    unfold f_ast_num_inc_proc_body;
+    rewrite <- H.
+  - specialize (leb_correct_conv _ _ H1); intros hz1.
+    rewrite hz1.
+    specialize (f_ast_num_inc_stmt_complete _ _ H0); auto.
+  - specialize (leb_correct_conv _ _ H2); intros hz1.
+    specialize (leb_correct_conv _ _ H3); intros hz2.
+    specialize (leb_correct_conv _ _ H4); intros hz3.
+    rewrite <- H in H0.
+    specialize (f_ast_num_inc_decls_complete _ _ _ H0); intros hz4.
+    specialize (f_ast_num_inc_stmt_complete _ _ H1); intros hz5.
+    rewrite hz1, hz2, hz4, hz5, hz3; simpl.
+    reflexivity.
+Qed.
+
+Lemma f_ast_num_inc_subprogram_correct: forall p max,
+    f_ast_num_inc_subprogram p = Some max ->
+    ast_num_inc_subprogram p max.
+Proof.
+    intros p;
+    functional induction (f_ast_num_inc_subprogram p);
+    intros max h1.
+    inversion h1.
+    constructor.
+    specialize (leb_complete_conv _ _ e0); auto.
+    specialize (f_ast_num_inc_proc_body_correct _ _ h1); auto.
+Qed.
+
+Lemma f_ast_num_inc_subprogram_complete: forall p max,
+    ast_num_inc_subprogram p max ->
+    f_ast_num_inc_subprogram p = Some max.
+Proof.
+    intros p max h1.
+    induction h1.
+    simpl.
+    specialize (leb_correct_conv _ _ H); intros hz1.
+    specialize (f_ast_num_inc_proc_body_complete _ _ H0); intros hz2.
+    rewrite hz1, hz2.
+    reflexivity.
+Qed.
+
+(* ===================================== *)
+
 (** ** Generate the run-time-check flags *)
 
 (** the run-time checks are stored in a list indexed with ast id number *)
@@ -535,6 +1777,15 @@ Inductive ast_nums_lt: check_points -> astnum -> Prop :=
         ast_nums_lt ((ast_num, ck) ::ls) n
     | lt2: forall n,
         ast_nums_lt nil n.
+
+(** the functional version for ast_nums_lt *)
+Function f_ast_nums_lt (ckp: check_points) (n: astnum): bool :=
+    match ckp with
+    | (ast_num, ck) :: tl => 
+        if leb n ast_num then false else f_ast_nums_lt tl n
+    | nil => true
+    end
+.
 
 Lemma ast_nums_lt_trans0: forall ls n n',
     ast_nums_lt ls n ->
@@ -615,6 +1866,381 @@ Inductive check_generator_stmt: check_points -> stmt -> check_points -> Prop :=
         check_generator_stmt ls2 c ls3 ->        
         check_generator_stmt ls1 (Swhile ast_num b c) ls3.
 
+
+Inductive check_generator_decl: check_points -> local_declaration -> check_points -> Prop :=
+    | CG_Decl0: forall d ls,
+        None = d.(local_init) ->
+        check_generator_decl ls d ls
+    | CG_Decl1: forall i d ls1 ls2,
+        Some i = d.(local_init) ->
+        check_generator_expr ls1 i ls2 ->
+        check_generator_decl ls1 d ls2.
+
+Inductive check_generator_decls: check_points -> list local_declaration -> check_points -> Prop :=
+    | CG_Decls_Empty: forall ls,
+        check_generator_decls ls nil ls
+    | CG_Decls: forall ls d ls'0 tl ls',
+        check_generator_decl ls d ls'0 ->
+        check_generator_decls ls'0 tl ls' ->
+        check_generator_decls ls (d :: tl) ls'.
+
+Inductive check_generator_proc_body: check_points -> procedure_body -> check_points -> Prop :=
+    | CG_Proc_Body: forall ls1 f ls2 ls3,
+        check_generator_decls ls1 f.(proc_loc_idents) ls2 ->
+        check_generator_stmt ls2 f.(proc_body) ls3 ->
+        check_generator_proc_body ls1 f ls3.
+
+Inductive check_generator_subprogram: check_points -> subprogram -> check_points -> Prop :=
+    | CG_Subprogram: forall ls1 f ls2 ast_num,
+        check_generator_proc_body ls1 f ls2 ->
+        check_generator_subprogram ls1 (Sproc ast_num f) ls2.
+
+
+(* =============================== *)
+
+(** Function for run-time checks generation according to checking rules *)
+
+Function f_check_flag (e: expr): option check_action :=
+    match e with
+    | Econst ast_num n => None
+    | Evar ast_num x => None
+    | Ebinop ast_num op e1 e2 => 
+        match op with
+        | Odiv => Some Do_Division_Check
+        | _ => None
+        end
+    | Eunop ast_num op e => None
+    end.
+
+Function f_check_generator_expr (ckp: check_points) (e: expr): check_points :=
+    match e with
+    | Econst ast_num n => ckp
+    | Evar ast_num x => ckp
+    | Ebinop ast_num op e1 e2 => 
+        match f_check_flag e with
+        | Some flag => 
+            let ckp' := f_check_generator_expr ((ast_num, flag) :: ckp) e1 in
+            f_check_generator_expr ckp' e2
+        | None => 
+            let ckp' := f_check_generator_expr ckp e1 in
+            f_check_generator_expr ckp' e2
+        end
+    | Eunop ast_num op e0 =>
+        f_check_generator_expr ckp e0
+    end.
+
+Function f_check_generator_stmt (ckp: check_points) (c: stmt): check_points :=
+    match c with
+    | Sassign ast_num x e => f_check_generator_expr ckp e
+    | Sseq ast_num c1 c2 =>
+        let ckp' := f_check_generator_stmt ckp c1 in
+        f_check_generator_stmt ckp' c2
+    | Sifthen ast_num b c0 => 
+        let ckp' := f_check_generator_expr ckp b in
+        f_check_generator_stmt ckp' c0
+    | Swhile ast_num b c0 => 
+        let ckp' := f_check_generator_expr ckp b in
+        f_check_generator_stmt ckp' c0
+    end.
+
+Function f_check_generator_decl (ckp: check_points) (d: local_declaration): check_points :=
+    match d.(local_init) with
+    | None => ckp
+    | Some i => f_check_generator_expr ckp i
+    end.
+
+Function f_check_generator_decls (ckp: check_points) (ds: list local_declaration): check_points :=
+    match ds with
+    | nil => ckp
+    | d :: tl => 
+        let ckp' := f_check_generator_decl ckp d in
+        f_check_generator_decls ckp' tl
+    end.
+
+Function f_check_generator_proc_body (ckp: check_points) (f: procedure_body): check_points :=
+    let ckp' := f_check_generator_decls ckp f.(proc_loc_idents) in
+    f_check_generator_stmt ckp' f.(proc_body).
+
+Function f_check_generator_subprogram (ckp: check_points) (p: subprogram): check_points :=
+    match p with
+    | Sproc ast_num f => f_check_generator_proc_body ckp f
+    end.
+
+
+(* =============================== *)
+
+(** Semantical equivalence between functional and relational style for run-time checks generation *)
+
+Lemma f_ast_nums_lt_correct: forall ckp n,
+    f_ast_nums_lt ckp n = true ->
+    ast_nums_lt ckp n.
+Proof.
+    induction ckp;
+    intros n h1.
+  - constructor.
+  - simpl in h1.
+    remember a as x.
+    destruct x.
+    remember (leb n a0) as y.
+    destruct y. inversion h1.
+    specialize (IHckp _ h1).
+    symmetry in Heqy. specialize (leb_complete_conv _ _ Heqy); intros hz1.
+    econstructor; auto.
+Qed.
+
+Lemma f_ast_nums_lt_complete: forall ckp n,
+    ast_nums_lt ckp n ->
+    f_ast_nums_lt ckp n = true.
+Proof.
+    induction ckp;
+    intros n h1.
+  - auto.
+  - remember a as x.
+    destruct x.
+    inversion h1; subst.
+    specialize (IHckp _ H3).
+    simpl.
+    specialize (leb_correct_conv _ _ H4); intros hz1.
+    rewrite hz1.
+    assumption.
+Qed.
+
+Lemma f_check_flag_correct: forall e ck,
+    f_check_flag e = ck ->
+    check_flag e ck.
+Proof.
+    intros e;
+    functional induction (f_check_flag e);
+    intros ck h1;
+    rewrite <- h1;
+    try constructor.
+  - destruct n; constructor.
+  - destruct op; inversion y;
+    unfold not; intros hz1; inversion hz1.
+Qed.
+
+Lemma f_check_flag_complete: forall e ck,
+    check_flag e ck ->
+    f_check_flag e = ck.
+Proof.
+    intros e ck h1.
+    induction h1;
+    auto.
+    destruct op; intuition.
+Qed.
+
+Lemma f_check_generator_expr_correct: forall ckp e ckp',
+    f_check_generator_expr ckp e = ckp' ->
+    check_generator_expr ckp e ckp'.
+Proof.
+    intros ckp e.
+    functional induction (f_check_generator_expr ckp e);
+    intros ckp' h1.
+  - rewrite <- h1.
+    constructor.
+  - rewrite <- h1.
+    constructor.
+  - specialize (IHc0 _ h1).
+    econstructor.
+    specialize (f_check_flag_correct _ _ e3); intros hz1.
+    exact hz1.
+    specialize (IHc (f_check_generator_expr ((ast_num, flag) :: ckp) e1)).
+    intuition.
+    exact H. assumption.
+  - specialize (IHc0 _ h1).
+    eapply CG_Ebinop_None.
+    specialize (f_check_flag_correct _ _ e3); auto.
+    specialize (IHc (f_check_generator_expr ckp e1)).
+    intuition.
+    exact H. assumption.
+  - specialize (IHc _ h1).
+    constructor.
+    assumption.
+Qed.
+
+Lemma f_check_generator_expr_complete: forall ckp e ckp',
+    check_generator_expr ckp e ckp' ->
+    f_check_generator_expr ckp e = ckp'.
+Proof.
+    intros ckp e ckp' h1.
+    induction h1;
+    simpl; auto.
+  - destruct op; inversion H; subst.
+    reflexivity.
+  - destruct op; inversion H; subst;
+    try rewrite IHh1_1, IHh1_2; auto.
+    destruct H1. reflexivity.
+Qed.
+
+Lemma f_check_generator_stmt_correct: forall ckp c ckp',
+    f_check_generator_stmt ckp c = ckp' ->
+    check_generator_stmt ckp c ckp'.
+Proof.
+    intros ckp c.
+    functional induction (f_check_generator_stmt ckp c);
+    intros ckp' h1.
+  - constructor.
+    specialize (f_check_generator_expr_correct _ _ _ h1); auto.
+  - specialize (IHc1 _ h1).
+    specialize (IHc0 (f_check_generator_stmt ckp c1)).
+    intuition.
+    econstructor.
+    exact H. assumption.
+  - specialize (IHc0 _ h1).
+    econstructor.
+    assert (hz1: f_check_generator_expr ckp b = f_check_generator_expr ckp b); auto.
+    specialize (f_check_generator_expr_correct _ _ _ hz1); intros hz2.
+    exact hz2.
+    assumption.
+  - specialize (IHc0 _ h1).
+    econstructor.
+    assert (hz1: f_check_generator_expr ckp b = f_check_generator_expr ckp b); auto.
+    specialize (f_check_generator_expr_correct _ _ _ hz1); intros hz2.
+    exact hz2.
+    assumption.
+Qed.
+
+Lemma f_check_generator_stmt_complete: forall ckp c ckp',
+    check_generator_stmt ckp c ckp' ->
+    f_check_generator_stmt ckp c = ckp'.
+Proof.
+    intros ckp c ckp' h1.
+    induction h1; simpl.
+  - specialize (f_check_generator_expr_complete _ _ _ H); 
+    auto.
+  - rewrite IHh1_1, IHh1_2.
+    reflexivity.
+  - specialize (f_check_generator_expr_complete _ _ _ H); intros hz1.
+    rewrite hz1.
+    assumption.
+  - specialize (f_check_generator_expr_complete _ _ _ H); intros hz1.
+    rewrite hz1.
+    assumption.
+Qed.
+
+Lemma f_check_generator_decl_correct: forall ckp d ckp',
+    f_check_generator_decl ckp d = ckp' ->
+    check_generator_decl ckp d ckp'.
+Proof.
+    intros ckp d;
+    functional induction (f_check_generator_decl ckp d);
+    intros ckp' h1.
+  - rewrite <- h1.
+    constructor.
+    auto.
+  - econstructor.
+    symmetry in e; exact e.
+    specialize (f_check_generator_expr_correct _ _ _ h1); auto.
+Qed.
+
+Lemma f_check_generator_decl_complete: forall ckp d ckp',
+    check_generator_decl ckp d ckp' ->
+    f_check_generator_decl ckp d = ckp'.
+Proof.
+    intros ckp d ckp' h1.
+    induction h1;
+    unfold f_check_generator_decl;
+    rewrite <- H; auto.
+    specialize (f_check_generator_expr_complete _ _ _ H0); auto.
+Qed.
+
+Lemma f_check_generator_decls_correct: forall tl ckp d ckp',
+    f_check_generator_decls ckp (d :: tl) = ckp' ->
+    check_generator_decls ckp (d :: tl) ckp'.
+Proof.
+    induction tl;
+    intros ckp d ckp' h1.
+  - simpl in h1.
+    specialize (f_check_generator_decl_correct _ _ _ h1); intros hz1.
+    econstructor.
+    exact hz1. constructor.
+  - simpl in h1.
+    specialize (IHtl _ _ _ h1).
+    econstructor.
+    assert (hz1: f_check_generator_decl ckp d = f_check_generator_decl ckp d); auto.
+    specialize (f_check_generator_decl_correct _ _ _ hz1); intros hz2.
+    exact hz2.
+    assumption.
+Qed.
+
+Lemma f_check_generator_decls_complete: forall tl ckp d ckp',
+    check_generator_decls ckp (d :: tl) ckp' ->
+    f_check_generator_decls ckp (d :: tl) = ckp'.
+Proof.
+    induction tl; 
+    intros ckp d ckp' h1;
+    simpl.
+  - inversion h1; subst.
+    inversion H4; subst.
+    specialize (f_check_generator_decl_complete _ _ _ H2); auto.
+  - inversion h1; subst.
+    specialize (IHtl _ _ _ H4).
+    specialize (f_check_generator_decl_complete _ _ _ H2); intros hz1.
+    rewrite hz1. assumption.
+Qed.
+
+Lemma f_check_generator_proc_body_correct: forall ckp f ckp',
+    f_check_generator_proc_body ckp f = ckp' ->
+    check_generator_proc_body ckp f ckp'.
+Proof.
+    intros ckp f;
+    functional induction (f_check_generator_proc_body ckp f);
+    intros ckp' h1.
+    remember (proc_loc_idents f) as x.
+    destruct x.
+    econstructor.
+    rewrite <- Heqx. constructor.
+    simpl in h1.
+    specialize (f_check_generator_stmt_correct _ _ _ h1); auto.
+    econstructor.
+    rewrite <- Heqx.
+    assert (hz1: (f_check_generator_decls ckp (l :: x)) = (f_check_generator_decls ckp (l :: x))); auto.
+    specialize (f_check_generator_decls_correct _ _ _ _ hz1); intros hz2.
+    exact hz2.
+    specialize (f_check_generator_stmt_correct _ _ _ h1); auto.
+Qed.
+
+Lemma f_check_generator_proc_body_complete: forall ckp f ckp',
+    check_generator_proc_body ckp f ckp' ->
+    f_check_generator_proc_body ckp f = ckp'.
+Proof.
+    intros ckp f ckp' h1.
+    induction h1.
+    remember (proc_loc_idents f) as x.
+    destruct x.
+  - inversion H; subst.
+    unfold f_check_generator_proc_body.
+    rewrite <- Heqx. simpl.
+    specialize (f_check_generator_stmt_complete _ _ _ H0); auto.
+  - unfold f_check_generator_proc_body.
+    rewrite <- Heqx. 
+    specialize (f_check_generator_decls_complete _ _ _ _ H); intros hz1.
+    rewrite hz1.
+    specialize (f_check_generator_stmt_complete _ _ _ H0); auto.
+Qed.
+
+Lemma f_check_generator_subprogram_correct: forall ckp p ckp',
+    f_check_generator_subprogram ckp p = ckp' ->
+    check_generator_subprogram ckp p ckp'.
+Proof.
+    intros ckp p;
+    functional induction (f_check_generator_subprogram ckp p);
+    intros ckp' h1.
+    constructor.
+    specialize (f_check_generator_proc_body_correct _ _ _ h1); auto.
+Qed.
+
+Lemma f_check_generator_subprogram_complete: forall ckp p ckp',
+    check_generator_subprogram ckp p ckp' ->
+    f_check_generator_subprogram ckp p = ckp'.
+Proof.
+    intros ckp p ckp' h1.
+    induction h1.
+    simpl.
+    specialize (f_check_generator_proc_body_complete _ _ _ H); auto.
+Qed.
+
+        
 (** ** Semantics with run-time-checks *)
 (*
 Inductive correct_flag_on_op: check_action -> binary_operation -> Prop :=
@@ -711,6 +2337,51 @@ Inductive eval_stmt_with_checks (cps: check_points): stack -> stmt -> state -> P
     | eval_While_False: forall s b ast_num c,
         eval_expr_with_checks cps s b (ValNormal (Bool false)) ->
         eval_stmt_with_checks cps s (Swhile ast_num b c) (SNormal s).
+
+(** variables declaration with initialization values are a little defferent from the assignments:
+    for variable declaration, we add the new declared variable with its initialization value to the initial stack,
+    because all declared variables have unique names;
+    for assignment, we update the initial stack by assigning new value to its component variable;
+*)
+Inductive eval_decl_with_checks (cps: check_points): stack -> local_declaration -> state -> Prop :=
+    | eval_Decl0: forall x d s,
+        x = d.(local_ident) ->
+        None = d.(local_init) ->
+        eval_decl_with_checks cps s d (SNormal ((x, Vundef) :: s))
+    | eval_Decl1: forall i d s,
+        Some i = d.(local_init) ->
+        eval_expr_with_checks cps s i ValException ->
+        eval_decl_with_checks cps s d SException
+    | eval_Decl2: forall x d i s v,
+        x = d.(local_ident) ->
+        Some i = d.(local_init) ->
+        eval_expr_with_checks cps s i (ValNormal v) ->
+        eval_decl_with_checks cps s d (SNormal ((x, Value v) :: s)).
+
+Inductive eval_decls_with_checks (cps: check_points): stack -> list local_declaration -> state -> Prop :=
+    | eval_Decls_Empty: forall s,
+        eval_decls_with_checks cps s nil (SNormal s)
+    | eval_Decls0: forall s d tl,
+        eval_decl_with_checks cps s d SException ->
+        eval_decls_with_checks cps s (d :: tl) SException
+    | eval_Decls1: forall s d s'0 tl s',
+        eval_decl_with_checks cps s d (SNormal s'0) ->
+        eval_decls_with_checks cps s'0 tl s' ->
+        eval_decls_with_checks cps s (d :: tl) s'.
+
+Inductive eval_proc_body_with_checks (cps: check_points): stack -> procedure_body -> state -> Prop :=
+    | eval_Proc_Body0: forall s f,
+        eval_decls_with_checks cps s f.(proc_loc_idents) SException ->
+        eval_proc_body_with_checks cps s f SException
+    | eval_Proc_Body1: forall s f s'0 s',
+        eval_decls_with_checks cps s f.(proc_loc_idents) (SNormal s'0) ->
+        eval_stmt_with_checks cps s'0 f.(proc_body) s' ->
+        eval_proc_body_with_checks cps s f s'.
+
+Inductive eval_subprogram_with_checks (cps: check_points): stack -> subprogram -> state -> Prop :=
+    | eval_Subprogram: forall s1 f s2 ast_num,
+        eval_proc_body_with_checks cps s1 f s2 ->
+        eval_subprogram_with_checks cps s1 (Sproc ast_num f) s2.
 
 
 (** some basic lemmas *)
@@ -820,6 +2491,819 @@ Proof.
     assert (hz: max1 + 1 <= get_ast_num_stmt c); intuition.
     specialize (ast_nums_lt_trans0 _ _ _ hz2 hz); intros hz3.
     specialize (IHh1 _ _ H11 hz3).
+    assumption.
+Qed.
+
+
+Lemma ast_num_bound_decl: forall d max,
+    ast_num_inc_decl d max ->
+    d.(local_astnum) <= max.
+Proof.
+    intros d max h.
+    induction h; simpl; intuition.
+    specialize (ast_num_bound_expr _ _ H1); intros hz1.
+    intuition.
+Qed.
+
+(** for declaration part with at least one declaration; *)
+Lemma ast_num_bound_decls: forall d tl max,
+    ast_num_inc_decls (d :: tl) max ->
+    d.(local_astnum) <= max.
+Proof.
+    intros.
+    remember (d :: tl) as ds.
+    revert Heqds. revert d tl.
+    induction H; intros;
+    inversion Heqds; subst.
+    apply (ast_num_bound_decl _ _ H); auto.
+    specialize (IHast_num_inc_decls d2 tl); intuition.
+    specialize (ast_num_bound_decl _ _ H); intros hz1. 
+    intuition.
+Qed.
+
+Lemma ast_num_max_decl: forall d max cks0 cks1,
+    ast_num_inc_decl d max ->
+    check_generator_decl cks0 d cks1 ->
+    ast_nums_lt cks0 d.(local_astnum) ->
+    ast_nums_lt cks1 (max + 1).
+Proof.
+    intros d max cks0 cks1 h1.
+    revert cks0 cks1.
+    induction h1;
+    intros cks0 cks1 h2 h3;
+    simpl in h3; inversion h2; subst.
+  - specialize (ast_num_bound_expr _ _ H1); intros hz1.
+    specialize (ast_nums_lt_trans _ _ _ h3 H3); intros hz2.
+    assert (hz3: get_ast_num_expr i < max + 1); intuition.
+    specialize (ast_nums_lt_trans _ _ _ hz2 hz3); intros hz4.
+    assumption.
+  - rewrite <- H0 in H4; inversion H4; subst.
+    specialize (ast_nums_lt_trans _ _ _ h3 H3); intros hz1.
+    specialize (ast_num_max_expr _ _ _ _ H1 H5 hz1); auto.
+  - assert (hz1: local_astnum d < local_astnum d + 1); intuition.
+    specialize (ast_nums_lt_trans _ _ _ h3 hz1); auto.
+  - rewrite <- H0 in H1; inversion H1.
+Qed.
+
+Lemma ast_num_max_decls: forall d tl max cks0 cks1,
+    ast_num_inc_decls (d :: tl) max ->
+    check_generator_decls cks0 (d :: tl) cks1 ->
+    ast_nums_lt cks0 d.(local_astnum) ->
+    ast_nums_lt cks1 (max + 1).
+Proof.
+    intros d tl max cks0 cks1 h1.
+    revert cks0 cks1.
+    remember (d :: tl) as ds. revert Heqds. revert d tl.
+    induction h1;
+    intros d'0 tl'0 h2 cks0 cks1 h3 h4;
+    inversion h2; subst.
+  - inversion h3; subst.
+    inversion H5; subst.
+    specialize (ast_num_max_decl _ _ _ _ H H3 h4); auto.
+  - specialize (IHh1 d2 tl); intuition.
+    inversion h3; subst.
+    specialize (ast_num_max_decl _ _ _ _ H H5 h4); intros hz1.
+    assert (hz2: n1 + 1 <= local_astnum d2); intuition.
+    specialize (ast_nums_lt_trans0 _ _ _ hz1 hz2); intros hz3.
+    specialize (H1 _ _ H7 hz3).
+    assumption.
+Qed.
+
+(* =============================== *)
+
+(** Functional semantics for expression and statement evaluation with checks as passed in parameters *)
+
+Function f_eval_expr_with_checks (ckp: check_points) (s: stack) (e: expr): return_val :=
+    match e with
+    | Econst ast_num n => ValNormal (eval_constant n)
+    | Evar ast_num x => 
+        match fetch x s with
+        | Some v => ValNormal v
+        | _ => ValAbnormal
+        end
+    | Ebinop ast_num op e1 e2 => 
+        match f_eval_expr_with_checks ckp s e1 with
+        | ValNormal v1 => 
+            match f_eval_expr_with_checks ckp s e2 with
+            | ValNormal v2 => 
+                match fetch_ck ast_num ckp with
+                | Some ck => 
+                    match f_do_check op v1 v2 with
+                    | Some true => f_eval_binexpr op v1 v2
+                    | Some false => ValException
+                    | _ => ValAbnormal
+                    end
+                | None => f_eval_binexpr op v1 v2
+                end
+            | ValException => ValException
+            | _ => ValAbnormal
+            end
+        | ValException => ValException
+        | _ => ValAbnormal
+        end
+    | Eunop ast_num op e0 =>
+        match f_eval_expr_with_checks ckp s e0 with
+        | ValNormal v => f_eval_unaryexpr op v
+        | ValException => ValException
+        | _ => ValAbnormal
+        end
+    end.
+
+Function f_eval_stmt_with_checks k (ckp: check_points) (s: stack) (c: stmt): state :=
+  match k with
+  | 0 => SUnterminated
+  | S k' =>
+    match c with
+    | Sassign ast_num x e =>
+        match f_eval_expr_with_checks ckp s e with
+        | ValNormal v => 
+            match update s x (Value v) with
+            | Some s1 => SNormal s1
+            | _ => SAbnormal
+            end
+        | ValException => SException
+        | _ => SAbnormal
+        end
+    | Sseq ast_num c1 c2 =>
+        match f_eval_stmt_with_checks k' ckp s c1 with
+        | SNormal s1 => f_eval_stmt_with_checks k' ckp s1 c2
+        | SException => SException
+        | SUnterminated => SUnterminated
+        | _ => SAbnormal
+        end
+    | Sifthen ast_num b c0 =>
+        match f_eval_expr_with_checks ckp s b with
+        | ValNormal (Bool true) => f_eval_stmt_with_checks k' ckp s c0
+        | ValNormal (Bool false) => SNormal s
+        | ValException => SException
+        | _ => SAbnormal
+        end
+    | Swhile ast_num b c0 =>
+        match f_eval_expr_with_checks ckp s b with
+        | ValNormal (Bool true) => 
+            match f_eval_stmt_with_checks k' ckp s c0 with
+            | SNormal s1 => f_eval_stmt_with_checks k' ckp s1 (Swhile ast_num b c0)
+            | SException => SException
+            | SUnterminated => SUnterminated
+            | _ => SAbnormal
+            end
+        | ValNormal (Bool false) => SNormal s
+        | ValException => SException
+        | _ => SAbnormal
+        end
+    end
+  end.
+
+Function f_eval_decl_with_checks (cps: check_points) (s: stack) (d: local_declaration): state :=
+    match d.(local_init) with
+    | Some i =>
+        match f_eval_expr_with_checks cps s i with
+        | ValNormal v => SNormal ((d.(local_ident), Value v) :: s)
+        | ValException => SException
+        | _ => SAbnormal
+        end
+    | None => SNormal ((d.(local_ident), Vundef) :: s)
+    end.
+
+Function f_eval_decls_with_checks (cps: check_points) (s: stack) (ds: list local_declaration): state :=
+    match ds with
+    | nil => SNormal s
+    | d :: tl =>
+        match f_eval_decl_with_checks cps s d with
+        | SNormal s1 => f_eval_decls_with_checks cps s1 tl
+        | SException => SException
+        | _ => SAbnormal
+        end
+    end.
+
+Function f_eval_proc_body_with_checks k (cps: check_points) (s: stack) (f: procedure_body): state :=
+    match f_eval_decls_with_checks cps s f.(proc_loc_idents) with
+    | SNormal s1 => f_eval_stmt_with_checks k cps s1 f.(proc_body)
+    | SException => SException
+    | _ => SAbnormal
+    end.
+
+Function f_eval_subprogram_with_checks k (cps: check_points) (s: stack) (p: subprogram): state :=
+    match p with
+    | Sproc ast_num f =>
+        f_eval_proc_body_with_checks k cps s f
+    end.
+
+(* ============================================ *)
+
+(** Semantical equivalence between the relatioinal semantics and functional semantics for
+    program evaluation with checks passed in as parameters; 
+*)
+
+Lemma f_eval_expr_with_checks_correct0: forall ckp s e v,
+    f_eval_expr_with_checks ckp s e = ValNormal v ->
+    eval_expr_with_checks ckp s e (ValNormal v).
+Proof.
+    intros ckp s e;
+    functional induction (f_eval_expr_with_checks ckp s e);
+    intros v' h1;
+    try match goal with
+    | [h: ValException = ValNormal ?v |- _] => inversion h
+    | [h: ValAbnormal = ValNormal ?v |- _] => inversion h
+    | [h: ValNormal ?v1 = ValNormal ?v2 |- _] => inversion h
+    end; subst; auto.
+  - constructor.
+    reflexivity.
+  - constructor.
+    assumption.
+  - specialize (IHr _ e3).
+    specialize (IHr0 _ e4).
+    econstructor.
+    exact IHr. exact IHr0.
+    exact e5.
+    specialize (f_do_check_correct _ _ _ _ e6); auto.
+    apply f_eval_binexpr_correct; auto.
+  - specialize (IHr _ e3).
+    specialize (IHr0 _ e4).
+    eapply eval_Binop5.
+    exact IHr. exact IHr0.
+    exact e5.
+    apply f_eval_binexpr_correct; auto.
+  - specialize (IHr _ e2).
+    econstructor.
+    exact IHr.
+    apply f_eval_unaryexpr_correct; auto.
+Qed.
+
+Lemma f_eval_expr_with_checks_correct1: forall ckp s e,
+    f_eval_expr_with_checks ckp s e = ValException ->
+    eval_expr_with_checks ckp s e ValException.
+Proof.
+    intros ckp s e;
+    functional induction (f_eval_expr_with_checks ckp s e);
+    intros h1;
+    try match goal with
+    |[h: ValNormal ?v = ValException |- _] => inversion h
+    |[h: ValAbnormal = ValException |- _] => inversion h
+    end.
+  - destruct v1, v2, op;
+    simpl in h1; inversion h1.
+  - specialize (f_eval_expr_with_checks_correct0 _ _ _ _ e3); intros hz1.
+    specialize (f_eval_expr_with_checks_correct0 _ _ _ _ e4); intros hz2.
+    eapply eval_Binop3.
+    apply hz1. apply hz2. apply e5.
+    apply f_do_check_correct; auto.
+  - destruct v1, v2, op;
+    simpl in h1; inversion h1.
+  - specialize (IHr0 e4).
+    eapply eval_Binop2.
+    specialize (f_eval_expr_with_checks_correct0 _ _ _ _ e3); intros hz1.
+    apply hz1. assumption.
+  - specialize (IHr e3).
+    constructor; assumption.
+  - destruct op, v; 
+    simpl in h1; inversion h1.
+  - specialize (IHr e2).
+    constructor; auto.
+Qed.
+
+Lemma f_eval_expr_with_checks_correct: forall ckp s e v,
+    (f_eval_expr_with_checks ckp s e = ValNormal v ->
+        eval_expr_with_checks ckp s e (ValNormal v)) /\ 
+    (f_eval_expr_with_checks ckp s e = ValException ->
+        eval_expr_with_checks ckp s e ValException).
+Proof.
+    intros.
+    split; intros.
+  - apply f_eval_expr_with_checks_correct0; 
+    auto.
+  - apply f_eval_expr_with_checks_correct1; 
+    auto.
+Qed.
+
+Lemma f_eval_expr_with_checks_complete: forall ckp s e v,
+    eval_expr_with_checks ckp s e v ->
+    f_eval_expr_with_checks ckp s e = v.
+Proof.
+    intros ckp s e v h1;
+    induction h1;
+    simpl;
+    repeat match goal with
+    | [h: ?x = ?y |- _] => rewrite h; clear h
+    end; auto.
+  - specialize (f_do_check_complete _ _ _ _ H0); intros hz1.
+    rewrite hz1.
+    reflexivity.
+  - specialize (f_do_check_complete _ _ _ _ H0); intros hz1.
+    rewrite hz1.
+    apply f_eval_binexpr_complete; auto.
+  - apply f_eval_binexpr_complete; auto.
+  - apply f_eval_unaryexpr_complete; auto.
+Qed.
+
+Ltac apply_expr_correct_lemma :=
+    match goal with
+    | |- eval_expr_with_checks ?ckp ?s ?e (ValNormal ?v) => 
+        apply f_eval_expr_with_checks_correct0
+    | |- eval_expr_with_checks ?ckp ?s ?e ValException =>
+        apply f_eval_expr_with_checks_correct1
+    end; auto.
+
+Ltac apply_expr_complete_lemma :=
+    match goal with
+    | h: eval_expr_with_checks ?ckp ?s ?e ?s' |- _ =>
+        rewrite (f_eval_expr_with_checks_complete _ _ _ _ h)
+    end; auto.
+
+Lemma f_eval_stmt_with_checks_correct0: forall k ckp s c s',
+    f_eval_stmt_with_checks k ckp s c = (SNormal s') ->
+    eval_stmt_with_checks ckp s c (SNormal s').
+Proof.
+    intros k ckp s c;
+    functional induction (f_eval_stmt_with_checks k ckp s c);
+    intros s' h1;
+    try match goal with
+    | [h: SUnterminated = SNormal ?s |- _] => inversion h
+    | [h: SException = SNormal ?s |- _] => inversion h
+    | [h: SAbnormal = SNormal ?s |- _] => inversion h
+    | [h: SNormal ?s1 = SNormal ?s2 |- _] => inversion h; subst
+    end.
+  - econstructor. 
+    apply_expr_correct_lemma.
+    apply e2.
+    assumption.
+  - specialize (IHs0 _ e1).
+    specialize (IHs1 _ h1).
+    econstructor.
+    apply IHs0. assumption.
+  - specialize (IHs0 _ h1).
+    econstructor.
+    apply_expr_correct_lemma.
+    assumption.
+  - eapply eval_Ifthen_False.
+    apply_expr_correct_lemma.
+  - specialize (IHs0 _ e2).
+    specialize (IHs1 _ h1).
+    econstructor.
+    apply_expr_correct_lemma.
+    apply IHs0. assumption.
+  - apply eval_While_False.
+    apply_expr_correct_lemma.
+Qed.
+
+Lemma f_eval_stmt_with_checks_correct1: forall k ckp s c,
+    f_eval_stmt_with_checks k ckp s c = SException ->
+    eval_stmt_with_checks ckp s c SException.
+Proof.
+    intros k ckp s c h1;
+    functional induction (f_eval_stmt_with_checks k ckp s c);
+    try match goal with
+    | [h: SUnterminated = SException |- _] => inversion h
+    | [h: SAbnormal = SException |- _] => inversion h
+    | [h: SNormal ?s1 = SException |- _] => inversion h
+    end.
+  - constructor.
+    apply_expr_correct_lemma.
+  - specialize (IHs1 h1).
+    specialize (f_eval_stmt_with_checks_correct0 _ _ _ _ _ e1); intros hz1.
+    eapply eval_Seq2.
+    apply hz1. assumption.
+  - specialize (IHs0 e1).
+    econstructor; auto.
+  - specialize (IHs0 h1).
+    apply eval_Ifthen_True.
+    apply_expr_correct_lemma.
+    assumption.
+  - constructor.
+    apply_expr_correct_lemma.
+  - specialize (IHs1 h1).
+    eapply eval_While_True2.
+    apply_expr_correct_lemma.
+    specialize (f_eval_stmt_with_checks_correct0 _ _ _ _ _ e2); intros hz1.
+    apply hz1.
+    assumption.
+  - specialize (IHs0 e2).
+    eapply eval_While_True1.
+    apply_expr_correct_lemma.
+    assumption.
+  - constructor.
+    apply_expr_correct_lemma.
+Qed.
+
+Lemma f_eval_stmt_with_checks_correct: forall k ckp s c s',
+    (f_eval_stmt_with_checks k ckp s c = (SNormal s') ->
+        eval_stmt_with_checks ckp s c (SNormal s')) /\
+    (f_eval_stmt_with_checks k ckp s c = SException ->
+        eval_stmt_with_checks ckp s c SException).
+Proof.
+    intros;
+    split; intros h1.
+  - apply f_eval_stmt_with_checks_correct0 with (k := k).
+    assumption.
+  - apply f_eval_stmt_with_checks_correct1 with (k := k).
+    assumption.
+Qed.
+
+(** Some help lemmas to prove f_eval_stmt_with_checks_complete; *)
+
+Lemma eval_stmt_with_checks_state : forall ckp s c s',
+        eval_stmt_with_checks ckp s c s' ->
+            (exists v, s' = SNormal v) \/ s' = SException.
+Proof.
+    intros ckp s c s' h.
+    induction h;
+    try match goal with
+    | [ |- (exists v, SNormal ?v1 = SNormal v) \/ _ ] => left; exists v1; reflexivity
+    | [ |- context [ _ \/ ?A = ?A ] ] => right; reflexivity
+    end; auto.
+Qed.
+
+Ltac apply_inv1 :=
+  match goal with
+    | H:SUnterminated = SNormal _ |- _ => inversion H
+    | H:SUnterminated = SException |- _ => inversion H
+    | H:SUnterminated = SAbnormal |- _ => inversion H
+    | H:SAbnormal = SNormal _ |- _ => inversion H
+    | H:SAbnormal = SException |- _ => inversion H
+    | H:SAbnormal = SUnterminated |- _ => inversion H
+    | H:SException = SNormal _ |- _ => inversion H
+    | H:SException = SAbnormal |- _ => inversion H
+    | H:SException = SUnterminated |- _ => inversion H
+    | H:SNormal _ = SUnterminated |- _ => inversion H
+    | H:SNormal _ = SException |- _ => inversion H
+    | H:SNormal _ = SAbnormal |- _ => inversion H
+    | H:SNormal _ = SNormal _ |- _ => inversion H;clear H;subst 
+    | H:update _ _ (Value _) = _ |- _ => rewrite H
+    | H:f_eval_expr_with_checks _ _ _ = _ |- _ => rewrite H
+    | H:f_eval_expr_with_checks _ _ = _ |- _ => rewrite H
+    | H: f_eval_stmt_with_checks _ _ _ _ = _ |- _ => rewrite H
+  end;subst;simpl;auto.
+
+Lemma f_eval_stmt_with_checks_fixpoint: forall k ckp s c s', 
+        f_eval_stmt_with_checks k ckp s c = SNormal s' ->
+        forall k':nat, (k <= k')%nat -> 
+            f_eval_stmt_with_checks k' ckp s c = SNormal s'.
+Proof.
+    intros k ckp s c.
+    functional induction (f_eval_stmt_with_checks k ckp s c); simpl; intros; subst; simpl; auto;
+    repeat progress apply_inv1.
+  - invle; 
+    repeat apply_inv1.
+  - invle.
+    + repeat apply_inv1.
+    + rewrite (IHs0 _ e1);auto with arith.
+  - invle; repeat apply_inv1. rewrite (IHs0 _ H);auto with arith.
+  - invle; repeat apply_inv1.
+  - invle; repeat apply_inv1. rewrite (IHs0 _ e2); auto with arith.
+  - invle; repeat apply_inv1.
+Qed.
+
+Lemma f_eval_stmt_with_checks_fixpoint_E: forall k ckp s c, 
+        f_eval_stmt_with_checks k ckp s c = SException ->
+        forall k':nat, (k <= k')%nat -> 
+            f_eval_stmt_with_checks k' ckp s c = SException.
+Proof.
+    intros k ckp s c.
+    functional induction (f_eval_stmt_with_checks k ckp s c); simpl; intros; subst; simpl; auto;
+    repeat progress apply_inv1.
+  - invle;
+    apply_inv1.
+  - invle;
+    repeat apply_inv1.
+    rewrite (f_eval_stmt_with_checks_fixpoint _ _ _ _ _ e1); auto with arith.
+  - invle;
+    repeat apply_inv1.
+    specialize (IHs0 e1). 
+    rewrite IHs0; auto with arith. 
+  - invle; 
+    repeat apply_inv1.
+    rewrite IHs0; auto with arith.
+  - invle;
+    repeat apply_inv1.
+  - invle; 
+    repeat apply_inv1. 
+    rewrite (f_eval_stmt_with_checks_fixpoint _ _ _ _ _ e2); auto with arith.
+  - invle; 
+    repeat apply_inv1.
+    rewrite (IHs0 e2); auto with arith.
+  - invle; 
+    repeat apply_inv1.
+Qed.
+
+Ltac kgreater1 :=
+  repeat match goal with
+           | h:f_eval_stmt_with_checks ?k ?ckp ?s ?c = SNormal ?s' |- context [f_eval_stmt_with_checks (?k + _) ?ckp ?s ?c] =>
+             rewrite (@f_eval_stmt_with_checks_fixpoint _ _ _ _ _ h);auto with arith
+           | h:f_eval_stmt_with_checks ?k ?ckp ?s ?c = SNormal ?s' |- context [f_eval_stmt_with_checks (_ + ?k) ?ckp ?s ?c] =>
+             rewrite (@f_eval_stmt_with_checks_fixpoint _ _ _ _ _ h);auto with arith
+           | h:f_eval_stmt_with_checks ?k ?ckp ?s ?c = SException |- context [f_eval_stmt_with_checks (?k + _) ?ckp ?s ?c] =>
+             rewrite (@f_eval_stmt_with_checks_fixpoint_E _ _ _ _ h);auto with arith
+           | h:f_eval_stmt_with_checks ?k ?ckp ?s ?c = SException |- context [f_eval_stmt_with_checks (_ + ?k) ?ckp ?s ?c] =>
+             rewrite (@f_eval_stmt_with_checks_fixpoint_E _ _ _ _ h);auto with arith
+         end.
+
+Ltac apply_rewrite1 := 
+    match goal with
+    | h: eval_expr_with_checks ?ckp ?s ?b ?s' |- _ => 
+        rewrite (f_eval_expr_with_checks_complete _ _ _ _ h)
+    | h: update _ _ _ = _ |- _ => rewrite h
+    end; auto.
+
+
+Lemma f_eval_stmt_with_checks_complete: forall ckp s c s',
+    eval_stmt_with_checks ckp s c s' ->
+    exists k, f_eval_stmt_with_checks k ckp s c = s'.
+Proof.
+    intros ckp s c s' h1;
+    induction h1.
+    (* 1. Sassign *)
+  - exists 1; simpl.
+    apply_rewrite1.
+  - exists 1; simpl.
+    repeat apply_rewrite1.
+    (* 2. Sseq *)
+  - destrIH.
+    exists (S k); simpl.
+    apply_inv1.
+  - destrIH.
+    exists (S (k0 + k)); simpl.
+    kgreater1.
+    specialize (eval_stmt_with_checks_state _ _ _ _ h1_2); intros hz1.
+    destruct hz1 as [hz2 | hz2].
+    + destrIH; rewrite hk1 in *; kgreater1.
+    + rewrite hz2 in *; kgreater1.
+  (* 3. Sifthen *)
+  - exists 1%nat; simpl.
+    apply_rewrite1.
+  - destrIH.
+    exists (S k); simpl.
+    apply_rewrite1.
+  (* 4. Swhile *)
+  - exists 1%nat; simpl.
+    apply_rewrite1.
+  - exists 1%nat; simpl.
+    apply_rewrite1.
+  - destrIH.
+    exists (S k); simpl.
+    apply_rewrite1.
+    apply_inv1.
+  - destrIH.
+    exists (S (k0+k)); simpl.
+    apply_rewrite1.
+    kgreater1.
+    specialize (eval_stmt_with_checks_state _ _ _ _ h1_2); intros hz1.
+    destruct hz1 as [hz2 | hz2].
+    + destrIH; rewrite hk1 in *; kgreater1.
+    + rewrite hz2 in *; kgreater1.
+  - exists 1%nat; simpl.
+    apply_rewrite1.
+Qed.
+
+Lemma f_eval_decl_with_checks_correct0: forall ckp s d s',
+    f_eval_decl_with_checks ckp s d = SNormal s' ->
+       eval_decl_with_checks ckp s d (SNormal s').
+Proof.
+    intros ckp s d;
+    functional induction (f_eval_decl_with_checks ckp s d);
+    intros s' h1;
+    try match goal with
+    | h: SAbnormal = SNormal ?s |- _ => inversion h
+    | h: SException = SNormal ?s |- _ => inversion h
+    | h: SNormal ?s1 = SNormal ?s2 |- _ => inversion h; subst
+    end; auto.
+  - econstructor; auto.
+    symmetry in e; apply e.
+    apply_expr_correct_lemma.
+  - econstructor; intuition.
+Qed.
+
+Lemma f_eval_decl_with_checks_correct1: forall ckp s d,
+    f_eval_decl_with_checks ckp s d = SException ->
+       eval_decl_with_checks ckp s d SException.
+Proof.
+    intros ckp s d;
+    functional induction (f_eval_decl_with_checks ckp s d);
+    intros h1;
+    try match goal with
+    | h: SAbnormal = SException |- _ => inversion h
+    | h: SNormal ?s = SException |- _ => inversion h
+    end; auto.
+    econstructor.
+    symmetry in e; apply e.
+    apply_expr_correct_lemma.
+Qed.
+
+Lemma f_eval_decl_with_checks_correct: forall ckp s d s',
+    (f_eval_decl_with_checks ckp s d = SNormal s' ->
+       eval_decl_with_checks ckp s d (SNormal s')) /\
+    (f_eval_decl_with_checks ckp s d = SException ->
+       eval_decl_with_checks ckp s d SException).
+Proof.
+    intros ckp s d s';
+    split; intros h1.
+  - apply f_eval_decl_with_checks_correct0; auto.
+  - apply f_eval_decl_with_checks_correct1; auto.
+Qed.
+
+Lemma f_eval_decl_with_checks_complete: forall ckp s d s',
+    eval_decl_with_checks ckp s d s' ->
+    f_eval_decl_with_checks ckp s d = s'.
+Proof.
+    intros ckp s d s' h1;
+    induction h1;
+    unfold f_eval_decl_with_checks;
+    rewrite <- H; try rewrite <- H0;
+    auto.
+  - apply_expr_complete_lemma.
+  - apply_expr_complete_lemma.
+Qed.
+
+Ltac apply_decl_correct_lemma :=
+    match goal with
+    | |- eval_decl_with_checks ?ckp ?s ?d (SNormal ?s') => apply f_eval_decl_with_checks_correct0
+    | |- eval_decl_with_checks ?ckp ?s ?d SException => apply f_eval_decl_with_checks_correct1
+    end; auto.
+
+Ltac apply_decl_complete_lemma :=
+    match goal with
+    | h: eval_decl_with_checks ?ckp ?s ?d ?s' |- _ => apply f_eval_decl_with_checks_complete
+    end; auto.
+
+Lemma f_eval_decls_with_checks_correct0: forall ckp s ds s',
+    f_eval_decls_with_checks ckp s ds = SNormal s' ->
+        eval_decls_with_checks ckp s ds (SNormal s').
+Proof.
+    intros ckp s ds; 
+    functional induction (f_eval_decls_with_checks ckp s ds);
+    intros s' h1;
+    try match goal with
+    | h: SAbnormal = SNormal ?s |- _ => inversion h
+    | h: SException = SNormal ?s |- _ => inversion h
+    | h: SNormal ?s1 = SNormal ?s2 |- _ => inversion h; subst
+    end; auto.
+  - constructor.
+  - specialize (IHs0 _ h1).
+    econstructor.
+    apply_decl_correct_lemma. apply e0.
+    assumption.
+Qed.
+
+Lemma f_eval_decls_with_checks_correct1: forall ckp s ds,
+    f_eval_decls_with_checks ckp s ds = SException ->
+        eval_decls_with_checks ckp s ds SException.
+Proof.
+    intros ckp s ds;
+    functional induction (f_eval_decls_with_checks ckp s ds);
+    intros h1;
+    try match goal with
+    | h: SAbnormal = SException |- _ => inversion h
+    | h: SNormal ?s = SException |- _ => inversion h
+    end; auto.
+  - specialize (IHs0 h1).
+    eapply eval_Decls1.
+    apply_decl_correct_lemma. apply e0.
+    assumption.
+  - constructor.
+    apply_decl_correct_lemma.
+Qed.
+
+Lemma f_eval_decls_with_checks_correct: forall ckp s ds s',
+    (f_eval_decls_with_checks ckp s ds = SNormal s' ->
+        eval_decls_with_checks ckp s ds (SNormal s')) /\
+    (f_eval_decls_with_checks ckp s ds = SException ->
+        eval_decls_with_checks ckp s ds SException).
+Proof.
+    intros;
+    split; intros h1.
+  - apply f_eval_decls_with_checks_correct0.
+    assumption.
+  - apply f_eval_decls_with_checks_correct1.
+    assumption.
+Qed.
+
+Lemma f_eval_decls_with_checks_complete: forall ckp s ds s',
+    eval_decls_with_checks ckp s ds s' ->
+    f_eval_decls_with_checks ckp s ds = s'.
+Proof.
+    intros ckp s ds s' h1.
+    induction h1;
+    simpl; auto.
+  - rewrite (f_eval_decl_with_checks_complete _ _ _ _ H).
+    reflexivity.
+  - rewrite (f_eval_decl_with_checks_complete _ _ _ _ H).
+    assumption.
+Qed.
+
+Lemma f_eval_proc_body_with_checks_correct0: forall k ckp s f s',
+    f_eval_proc_body_with_checks k ckp s f = SNormal s' ->
+        eval_proc_body_with_checks ckp s f (SNormal s').
+Proof.
+    intros k ckp s f;
+    functional induction (f_eval_proc_body_with_checks k ckp s f);
+    intros s' h1;
+    try match goal with
+    |h: SException = SNormal ?s |- _ => inversion h
+    |h: SAbnormal = SNormal ?s |- _ => inversion h
+    end.
+  - econstructor.
+    apply f_eval_decls_with_checks_correct0.
+    apply e.
+    apply f_eval_stmt_with_checks_correct0 with (k := k).
+    assumption.
+Qed.
+
+Lemma f_eval_proc_body_with_checks_correct1: forall k ckp s f,
+    f_eval_proc_body_with_checks k ckp s f = SException ->
+        eval_proc_body_with_checks ckp s f SException.
+Proof.
+    intros k ckp s f;
+    functional induction (f_eval_proc_body_with_checks k ckp s f);
+    intros h1;
+    try match goal with
+    |h: SNormal ?s = SException |- _ => inversion h
+    |h: SAbnormal = SException |- _ => inversion h
+    end.
+  - eapply eval_Proc_Body1.
+    apply f_eval_decls_with_checks_correct0. 
+    apply e.
+    apply f_eval_stmt_with_checks_correct1 with (k := k).
+    assumption.
+  - constructor.
+    apply f_eval_decls_with_checks_correct1.
+    assumption.
+Qed.
+
+Lemma f_eval_proc_body_with_checks_correct: forall k ckp s f s',
+    (f_eval_proc_body_with_checks k ckp s f = SNormal s' ->
+        eval_proc_body_with_checks ckp s f (SNormal s')) /\
+    (f_eval_proc_body_with_checks k ckp s f = SException ->
+        eval_proc_body_with_checks ckp s f SException).
+Proof.
+    intros;
+    split; intros h1.
+  - apply f_eval_proc_body_with_checks_correct0 with (k := k).
+    assumption.
+  - apply f_eval_proc_body_with_checks_correct1 with (k := k).
+    assumption.
+Qed.
+
+Lemma f_eval_proc_body_with_checks_complete: forall ckp s f s',
+    eval_proc_body_with_checks ckp s f s' ->
+    exists k, f_eval_proc_body_with_checks k ckp s f = s'.
+Proof.
+    intros ckp s f s' h1;
+    induction h1;
+    unfold f_eval_proc_body_with_checks.
+  - rewrite (f_eval_decls_with_checks_complete _ _ _ _ H).
+    exists 1%nat.
+    reflexivity.
+  - rewrite (f_eval_decls_with_checks_complete _ _ _ _ H).
+    apply f_eval_stmt_with_checks_complete.
+    assumption.
+Qed.
+
+Lemma f_eval_subprogram_with_checks_correct0: forall k ckp s p s',
+    f_eval_subprogram_with_checks k ckp s p = SNormal s' ->
+        eval_subprogram_with_checks ckp s p (SNormal s').
+Proof.
+    intros k ckp s p;
+    functional induction (f_eval_subprogram_with_checks k ckp s p);
+    intros s' h1.
+  - constructor.
+    apply f_eval_proc_body_with_checks_correct0 with (k := k);
+    auto.
+Qed.
+
+Lemma f_eval_subprogram_with_checks_correct1: forall k ckp s p,
+    f_eval_subprogram_with_checks k ckp s p = SException ->
+        eval_subprogram_with_checks ckp s p SException.
+Proof.
+    intros k ckp s p;
+    functional induction (f_eval_subprogram_with_checks k ckp s p);
+    intros h1.
+  - constructor.
+    apply f_eval_proc_body_with_checks_correct1 with (k := k);
+    auto.
+Qed.
+
+Lemma f_eval_subprogram_with_checks_correct: forall k ckp s p s',
+    (f_eval_subprogram_with_checks k ckp s p = SNormal s' ->
+        eval_subprogram_with_checks ckp s p (SNormal s')) /\
+    (f_eval_subprogram_with_checks k ckp s p = SException ->
+        eval_subprogram_with_checks ckp s p SException).
+Proof.
+    intros;
+    split; intros h1.
+  - apply f_eval_subprogram_with_checks_correct0 with (k := k);
+    auto.
+  - apply f_eval_subprogram_with_checks_correct1 with (k := k);
+    auto.
+Qed.
+
+Lemma f_eval_subprogram_with_checks_complete: forall ckp s p s',
+    eval_subprogram_with_checks ckp s p s' ->
+    exists k, f_eval_subprogram_with_checks k ckp s p = s'.
+Proof.
+    intros ckp s p s' h1;
+    induction h1.
+  - specialize (f_eval_proc_body_with_checks_complete _ _ _ _ H); intros hz1.
+    destrIH.
+    exists k; unfold f_eval_subprogram_with_checks.
     assumption.
 Qed.
 
