language_formal/spark2014_semantics/util.v
@@ -75,4 +75,3 @@ Ltac distr_qualifier :=
 
 
 
-
